Utils.thy
@@ -1,5 +1,7 @@
 theory Utils
-imports "Propositional_Proof_Systems.Formulas"
+  imports
+    "Propositional_Proof_Systems.Sema"
+    "AI_Planning_Languages_Semantics.PDDL_STRIPS_Semantics"
 begin
 
 (* formula helpers *)
@@ -14,17 +16,7 @@ fun only_conj :: "'a formula \<Rightarrow> bool" where
   "only_conj (_ \<^bold>\<or> _) \<longleftrightarrow> False" |
   "only_conj (_ \<^bold>\<rightarrow> _) \<longleftrightarrow> False"
 
-fun disj_fmlas :: "'a formula list \<Rightarrow> 'a formula" where
-  "disj_fmlas [] = Bot" |
-  "disj_fmlas [f] = f" |
-  "disj_fmlas (f # fs) = f \<^bold>\<or> disj_fmlas fs"
-
-fun conj_fmlas :: "'a formula list \<Rightarrow> 'a formula" where
-  "conj_fmlas [] = \<^bold>\<not> \<bottom>" |
-  "conj_fmlas [f] = f" |
-  "conj_fmlas (f # fs) = f \<^bold>\<and> conj_fmlas fs"
-
-(* lemmas *)
+(* random lemmas *)
 
 lemma map_of_in_R_iff: "x \<in> fst ` set m \<longleftrightarrow> (\<exists>y. map_of m x = Some y)"
   by (metis map_of_eq_None_iff not_None_eq)
@@ -57,5 +49,128 @@ lemma conj_split_7:
   assumes "A \<and> B \<and> C \<and> D \<and> E \<and> F \<and> G"
   shows "A" "B" "C" "D" "E" "F" "G"
   using assms by simp_all
+
+subsection \<open> Static predicates \<close>
+
+
+
+definition fmla_preds :: "'ent atom formula \<Rightarrow> predicate set" where
+  "fmla_preds F = {p | p xs. predAtm p xs \<in> atoms F}"
+lemma fmla_preds_simps [simp]:
+  "fmla_preds (Atom (predAtm p xs)) = {p}"
+  "fmla_preds (Atom (Eq a b)) = {}"
+  "fmla_preds \<bottom> = {}"
+  "fmla_preds (\<^bold>\<not> F) = fmla_preds F"
+  "fmla_preds (F1 \<^bold>\<and> F2) = fmla_preds F1 \<union> fmla_preds F2"
+  "fmla_preds (F1 \<^bold>\<or> F2) = fmla_preds F1 \<union> fmla_preds F2"
+  "fmla_preds (F1 \<^bold>\<rightarrow> F2) = fmla_preds F1 \<union> fmla_preds F2"
+    apply (force simp: fmla_preds_def)
+   apply (force simp: fmla_preds_def)
+   apply (force simp: fmla_preds_def)
+   apply (force simp: fmla_preds_def)
+   apply (force simp: fmla_preds_def)
+   apply (force simp: fmla_preds_def)
+  apply (force simp: fmla_preds_def)
+  done
+
+lemma "p \<notin> fmla_preds F \<Longrightarrow> predAtm p xd \<notin> atoms F"
+  by (simp add: fmla_preds_def)
+
+lemma map_preserves_fmla_preds: "fmla_preds F = fmla_preds ((map_formula \<circ> map_atom) f F)"
+proof (induction F)
+  case (Atom x)
+  thus ?case by (cases x) simp_all
+qed auto
+
+
+thm irrelevant_atom
+
+subsection \<open> STRIPS Formulas \<close>
+
+text \<open>The lemma \<open>pn_atoms_updates\<close> is in a very unfortunate form, so I have to split it.\<close>
+
+lemma prod_unions_alt: "prod_unions (a, b) (c, d) = (a \<union> c, b \<union> d)"
+  using prod_unions_def by auto
+
+lemma snd_prod_unions: "snd (prod_unions A B) = snd A \<union> snd B"
+  apply (induction A; induction B)
+  by (simp_all add: prod_unions_alt)
+
+lemma fst_prod_unions: "fst (prod_unions A B) = fst A \<union> fst B"
+  apply (induction A; induction B)
+  by (simp_all add: prod_unions_alt)
+
+lemma pn_atoms_updates_split: "(p \<notin> snd (pn_atoms F) \<longrightarrow>
+    ((M \<Turnstile> F \<longrightarrow> M(p := True) \<Turnstile> F)
+    \<and> (\<not>(M \<Turnstile> F) \<longrightarrow> \<not>M(p := False) \<Turnstile> F))) \<and>
+   (p \<notin> fst (pn_atoms F) \<longrightarrow>
+    ((M \<Turnstile> F \<longrightarrow> M(p := False) \<Turnstile> F)
+    \<and> (\<not>(M \<Turnstile> F) \<longrightarrow> \<not>M(p := True) \<Turnstile> F)))"
+  (is "(?notn \<longrightarrow> (?A F\<and> ?B)) \<and> (?notp \<longrightarrow> (?C \<and> ?D))")
+proof (induction F)
+  case (And F1 F2)
+    (* TODO: can I just use "intro conjI; intro: impI" here to automatically create assumptions and split the goal? *)
+  { assume "p \<notin> snd (pn_atoms (F1 \<^bold>\<and> F2))"
+    hence "p \<notin> snd (pn_atoms F1) \<and> p \<notin> snd (pn_atoms F2)"
+      using snd_prod_unions pn_atoms.simps(4) by (metis UnCI)
+    hence "(M \<Turnstile> F1 \<^bold>\<and> F2 \<longrightarrow> M(p := True) \<Turnstile> F1 \<^bold>\<and> F2) \<and> (\<not> M \<Turnstile> F1 \<^bold>\<and> F2 \<longrightarrow> \<not> M(p := False) \<Turnstile> F1 \<^bold>\<and> F2)"
+      using And.IH formula_semantics.simps(4) by blast }
+  moreover { assume "p \<notin> fst (pn_atoms (F1 \<^bold>\<and> F2))"
+    hence "p \<notin> fst (pn_atoms F1) \<and> p \<notin> fst (pn_atoms F2)"
+      using fst_prod_unions pn_atoms.simps(4) by (metis UnCI)
+    hence "(M \<Turnstile> F1 \<^bold>\<and> F2 \<longrightarrow> M(p := False) \<Turnstile> F1 \<^bold>\<and> F2) \<and> (\<not> M \<Turnstile> F1 \<^bold>\<and> F2 \<longrightarrow> \<not> M(p := True) \<Turnstile> F1 \<^bold>\<and> F2)"
+      using And.IH formula_semantics.simps(4) by blast }
+  ultimately show ?case by blast
+next
+  case (Or F1 F2)
+  { assume "p \<notin> snd (pn_atoms (F1 \<^bold>\<or> F2))"
+    hence "p \<notin> snd (pn_atoms F1) \<and> p \<notin> snd (pn_atoms F2)"
+      using snd_prod_unions pn_atoms.simps(5) by (metis UnCI)
+    hence "(M \<Turnstile> F1 \<^bold>\<or> F2 \<longrightarrow> M(p := True) \<Turnstile> F1 \<^bold>\<or> F2) \<and> (\<not> M \<Turnstile> F1 \<^bold>\<or> F2 \<longrightarrow> \<not> M(p := False) \<Turnstile> F1 \<^bold>\<or> F2)"
+      using Or.IH formula_semantics.simps(5) by blast }
+  moreover { assume "p \<notin> fst (pn_atoms (F1 \<^bold>\<or> F2))"
+    hence "p \<notin> fst (pn_atoms F1) \<and> p \<notin> fst (pn_atoms F2)"
+      using fst_prod_unions pn_atoms.simps(5) by (metis UnCI)
+    hence "(M \<Turnstile> F1 \<^bold>\<or> F2 \<longrightarrow> M(p := False) \<Turnstile> F1 \<^bold>\<or> F2) \<and> (\<not> M \<Turnstile> F1 \<^bold>\<or> F2 \<longrightarrow> \<not> M(p := True) \<Turnstile> F1 \<^bold>\<or> F2)"
+      using Or.IH formula_semantics.simps(5) by blast }
+  ultimately show ?case by blast
+next
+  case (Imp F1 F2)
+  note Imp.IH
+  { assume "p \<notin> snd (pn_atoms (F1 \<^bold>\<rightarrow> F2))"
+    hence "p \<notin> fst (pn_atoms F1) \<and> p \<notin> snd (pn_atoms F2)"
+      using snd_prod_unions pn_atoms.simps(6) UnCI by (metis snd_swap)
+    hence "(M \<Turnstile> F1 \<^bold>\<rightarrow> F2 \<longrightarrow> M(p := True) \<Turnstile> F1 \<^bold>\<rightarrow> F2) \<and> (\<not> M \<Turnstile> F1 \<^bold>\<rightarrow> F2 \<longrightarrow> \<not> M(p := False) \<Turnstile> F1 \<^bold>\<rightarrow> F2)"
+      using Imp.IH formula_semantics.simps(6) by blast }
+  moreover { assume "p \<notin> fst (pn_atoms (F1 \<^bold>\<rightarrow> F2))"
+    hence "p \<notin> snd (pn_atoms F1) \<and> p \<notin> fst (pn_atoms F2)"
+      using fst_prod_unions pn_atoms.simps(6) UnCI by (metis fst_swap)
+    hence "(M \<Turnstile> F1 \<^bold>\<rightarrow> F2 \<longrightarrow> M(p := False) \<Turnstile> F1 \<^bold>\<rightarrow> F2) \<and> (\<not> M \<Turnstile> F1 \<^bold>\<rightarrow> F2 \<longrightarrow> \<not> M(p := True) \<Turnstile> F1 \<^bold>\<rightarrow> F2)"
+      using Imp.IH formula_semantics.simps(6) by blast }
+  ultimately show ?case by blast
+qed simp_all
+
+(* this now follows *)
+thm pn_atoms_updates
+lemma "p \<notin> snd (pn_atoms F) \<Longrightarrow> n \<notin> fst (pn_atoms F) \<Longrightarrow>
+  ((M \<Turnstile> F \<longrightarrow> (M(p := True) \<Turnstile> F \<and> M(n := False) \<Turnstile> F)))
+\<and> ((\<not>(M \<Turnstile> F)) \<longrightarrow> \<not>(M(n := True) \<Turnstile> F) \<and> \<not>(M(p := False) \<Turnstile> F))"
+  using pn_atoms_updates_split by metis
+
+lemma p_atoms_updates:
+  assumes "p \<notin> snd (pn_atoms F)"
+  shows "M \<Turnstile> F \<longrightarrow> M(p := True) \<Turnstile> F"
+        "\<not>(M \<Turnstile> F) \<longrightarrow> \<not>M(p := False) \<Turnstile> F"
+  apply (metis assms pn_atoms_updates_split)
+  by (metis assms pn_atoms_updates_split)
+
+lemma n_atoms_updates:
+  assumes "p \<notin> fst (pn_atoms F)"
+  shows "M \<Turnstile> F \<longrightarrow> M(p := False) \<Turnstile> F"
+        "\<not>(M \<Turnstile> F) \<longrightarrow> \<not>M(p := True) \<Turnstile> F"
+  apply (metis assms pn_atoms_updates_split)
+  by (metis assms pn_atoms_updates_split)
+
+
 
 end
